project/inductive/inductive_graph_theory.v
@@ -42,7 +42,7 @@ Qed.
 Check NatMap.elements .
 
 
-
+(* Notive, how In + [] is basically used as a set. Also possibly provide no duplicates proofs *) 
 
 (* Helper lemma for converting an In (of a map) to an InA, which will eventually be turned to a NatMap.In (which has useful lemmas)  *)
 Lemma _In_map_fst_InA : forall (A B: Type) (x : LNode A) (l : list (Node * (Context' A B))),
@@ -135,21 +135,381 @@ Proof.
   - reflexivity.
 Qed.
 
+Lemma _updAdj_does_not_change_key_set : forall (A B : Type) (adj : Adj B) (f : B -> Context' A B -> Context' A B) (ig : IG A B) (x : Node), 
+  In x (map fst (IG_labNodes (_updAdj adj f ig))) <-> In x (map fst (IG_labNodes ig)).
+Proof.
+  intros. unfold _updAdj.
+  induction adj.
+  - simpl. reflexivity.
+  - simpl. destruct a. rewrite _updateEntry_does_not_change_key_set. rewrite <- IHadj. reflexivity.
+Qed.
 
 
+(* util *)
+Require Import MyProject.project.util.util.
+
+Check _addSucc.
+Check _addSucc 3.
+Check _updateEntry.
+
+(* This is just a lightly harder version of the 2 proofs above *)
+Lemma _updateEntry_addSucc_does_not_change_lab_nodes : forall (A B : Type) (node : Node) (whose : Node) (l : B) (ig : IG A B) (x : LNode A),
+  In x (IG_labNodes (_updateEntry node (_addSucc whose l) ig)) <-> In x (IG_labNodes ig).    
+Proof.
+  intros. unfold _updateEntry. unfold _addSucc. 
+  destruct (NatMap.find node ig) eqn:isIn.
+  - destruct c as [[froms label] tos]. rewrite !_In_labNodes_is_InMap. split; intros.
+    + destruct H as [fromss [toss H]]. apply WF.add_mapsto_iff in H. destruct H.
+      -- exists froms, tos. destruct H. inversion H0. subst. apply WF.find_mapsto_iff. assumption.
+      -- firstorder.
+    + firstorder. bdestruct ((fst x) =? node).
+      -- subst. exists froms, ((l, whose) :: tos). apply WF.add_mapsto_iff. left. split.
+        ++ reflexivity.
+        ++ destruct x. simpl in *. apply WF.find_mapsto_iff in isIn. assert ((froms, label, tos) = (x0, a, x1)). {
+          apply (WF.MapsTo_fun isIn).
+          assumption.
+        }
+        inversion H0. firstorder.
+      -- exists x0, x1. apply WF.add_mapsto_iff. right. split.
+        ++ lia.
+        ++ assumption.
+  - reflexivity.
+Qed.
+
+
+
+Lemma _updAdj_addSucc_does_not_change_lab_nodes : forall (A B : Type) (node : Node) (adj : Adj B) (ig : IG A B) (x : LNode A), 
+  In x (IG_labNodes (_updAdj adj (_addSucc node) ig)) <-> In x (IG_labNodes ig).
+Proof.
+  intros. unfold _updAdj.
+  induction adj.
+  - simpl. reflexivity.
+  - simpl. destruct a. rewrite _updateEntry_addSucc_does_not_change_lab_nodes. rewrite <- IHadj. reflexivity.
+Qed.
+
+(* this is just a pallete- swap version of the two proofs above *)
+Lemma _updateEntry_addPred_does_not_change_lab_nodes : forall (A B : Type) (node : Node) (whose : Node) (l : B) (ig : IG A B) (x : LNode A),
+  In x (IG_labNodes (_updateEntry node (_addPred whose l) ig)) <-> In x (IG_labNodes ig).    
+Proof.
+  intros. unfold _updateEntry. unfold _addPred. 
+  destruct (NatMap.find node ig) eqn:isIn.
+  - destruct c as [[froms label] tos]. rewrite !_In_labNodes_is_InMap. split; intros.
+    + destruct H as [fromss [toss H]]. apply WF.add_mapsto_iff in H. destruct H.
+      -- exists froms, tos. destruct H. inversion H0. subst. apply WF.find_mapsto_iff. assumption.
+      -- firstorder.
+    + firstorder. bdestruct ((fst x) =? node).
+      -- subst. exists ((l, whose) :: froms), tos. apply WF.add_mapsto_iff. left. split. 
+        ++ reflexivity.
+        ++ destruct x. simpl in *. apply WF.find_mapsto_iff in isIn. assert ((froms, label, tos) = (x0, a, x1)). {
+          apply (WF.MapsTo_fun isIn).
+          assumption.
+        }
+        inversion H0. firstorder.
+      -- exists x0, x1. apply WF.add_mapsto_iff. right. split.
+        ++ lia.
+        ++ assumption.
+  - reflexivity.
+Qed.
+
+Lemma _updAdj_addPred_does_not_change_lab_nodes : forall (A B : Type) (node : Node) (adj : Adj B) (ig : IG A B) (x : LNode A), 
+  In x (IG_labNodes (_updAdj adj (_addPred node) ig)) <-> In x (IG_labNodes ig).
+Proof.
+  intros. unfold _updAdj.
+  induction adj.
+  - simpl. reflexivity.
+  - simpl. destruct a. rewrite _updateEntry_addPred_does_not_change_lab_nodes. rewrite <- IHadj. reflexivity.
+Qed.
+
+
+Lemma IG_add_adds_node : forall (A B : Type) (context : Context A B) (ig : IG A B) (x : LNode A),
+  In x (IG_labNodes (add context ig)) <-> let '(_, node, label, _) := context in In x ((if NatMap.mem node ig then [] else [(node, label)]) ++ IG_labNodes ig).
+Proof.
+  intros. simpl.
+  destruct context as [[[froms node] label] tos]. unfold add.
+  destruct (NatMap.mem node ig) eqn:cond; simpl.
+  - reflexivity.
+  - rewrite _updAdj_addSucc_does_not_change_lab_nodes. rewrite _updAdj_addPred_does_not_change_lab_nodes.
+    rewrite !_In_labNodes_is_InMap. 
+  
+  split; intros.
+    + destruct H as [fromss [toss H]]. apply WF.add_mapsto_iff in H. destruct H.
+      -- left. destruct x. destruct H. inversion H0. simpl in *. subst. reflexivity.
+      -- right. destruct H. firstorder.
+    + destruct H.
+      -- exists froms, tos. apply WF.add_mapsto_iff. left. destruct x. inversion H. simpl in *. subst. auto.
+      -- destruct H as [fromss [toss H]]. exists fromss, toss. apply WF.add_mapsto_iff. right. split.
+        ++ unfold not. intros. destruct x. simpl in *. subst. assert (NatMap.In n ig). {
+            firstorder.          
+        } apply NatMap.mem_1 in H0. rewrite H0 in cond. discriminate cond.
+        ++ assumption.
+Qed.
+
+
+
+
+
+
+Lemma _insNode_any_ins_node : forall (A B : Type) (node : LNode A) (ig : IG A B) (x : LNode A),
+  In x (IG_labNodes (_insNode node ig)) <-> In x ((if NatMap.mem (fst node) ig then [] else [node]) ++ IG_labNodes ig).
+Proof.
+  intros. simpl.
+  destruct node.
+  pose proof (IG_add_adds_node _ B (nil, n, a, nil)).
+  unfold _insNode.
+  rewrite H.
+  simpl.
+  reflexivity.
+Qed.
+
+
+
+
+
+Definition filterAndRemoveDuplicates (l : list nat) : list nat :=
+  fold_right (fun (k : nat) (acc : list nat) => if (k =? 420) || existsb (Nat.eqb k ) acc then acc else k :: acc) [] l.
+
+
+Compute filterAndRemoveDuplicates [1 ; 2 ; 3 ; 1 ; 2 ; 3; 420].
+
+Check Forall.
+Check NoDupA.
+
+
+Lemma _mem_different_insNodes : forall (A B : Type) (n : Node) (a : A) (nodes : list (LNode A)) (ig : IG A B),
+  ~ InA (fun x y : NatSet.Node * A => fst x = fst y) (n, a) nodes ->
+  NatMap.mem n (_insNodes nodes ig) = NatMap.mem n ig.
+Proof.
+  intros. induction nodes.
+  - simpl. reflexivity.
+  - simpl. destruct a0. assert (~ InA (fun x y : NatSet.Node * A => fst x = fst y) (n, a) nodes). {
+    firstorder.
+    } apply IHnodes in H0.
+    assert (n <> n0). {
+      firstorder.
+    }
+    
+    destruct (NatMap.mem n ig) eqn:HH.
+    + apply WF.mem_in_iff. apply WF.mem_in_iff in H0. simpl. destruct (NatMap.mem n0 (_insNodes nodes ig)).
+      -- assumption.
+      -- apply WF.add_in_iff. right. assumption.
+    + apply WF.not_mem_in_iff. apply WF.not_mem_in_iff in H0. simpl. unfold not. intros. destruct (NatMap.mem n0 (_insNodes nodes ig)).
+      -- firstorder.
+      -- apply WF.add_in_iff in H2. destruct H2.
+        ++ auto.
+        ++ firstorder.
+Qed.
+
+
+
+
+Lemma _insNodes_any_ins_all_nodes : forall (A B : Type) (nodes : list (LNode A)) (ig : IG A B) (x : LNode A),
+  NoDupA (fun x y => fst x = fst y) nodes ->
+  In x (IG_labNodes (_insNodes nodes ig)) <-> In x (filter (fun '(n, _) => negb (NatMap.mem n ig)) nodes ++ IG_labNodes ig).
+Proof.
+  intros. induction nodes.
+    - simpl. reflexivity.
+    - simpl. inversion H. apply IHnodes in H3. rewrite _insNode_any_ins_node. destruct a. simpl.
+      apply (_mem_different_insNodes _ B _ _ _ ig) in H2.
+      rewrite H2.
+      destruct (NatMap.mem n ig) eqn:HH.
+
+      + simpl. rewrite H3. reflexivity.
+      + simpl. rewrite H3. reflexivity.
+Qed.
+
+
+
+Lemma IG_match_returns_node : forall (A B : Type) (query hit : Node) (ig i : IG A B) (froms tos : Adj B) (l : A),
+  IG_match query ig = (Some (froms, hit, l, tos), i) -> query = hit.
+Proof.
+  intros. unfold IG_match in H. destruct (NatMap.find query ig).
+  - unfold _cleanSplit in H. destruct c as [[fromss label] toss]. inversion H. reflexivity. 
+  - inversion H.
+Qed.
+  
+
+
+(* this is just a pallete- swap version of the 4 _updateEntry  proofs further above *)
+
+(* this is just a pallete- swap version of the 4 _updateEntry  proofs further above *)
+Lemma _updateEntry_filter_clearSucc_does_not_change_lab_nodes : forall (A B : Type) (node : Node) (whose : Node) (l : B) (ig : IG A B) (x : LNode A),
+  In x (IG_labNodes (_updateEntry node (_addPred whose l) ig)) <-> In x (IG_labNodes ig).   
+Proof.
+  (* intros. unfold _updateEntry. unfold _addPred. 
+  destruct (NatMap.find node ig) eqn:isIn.
+  - destruct c as [[froms label] tos]. rewrite !_In_labNodes_is_InMap. split; intros.
+    + destruct H as [fromss [toss H]]. apply WF.add_mapsto_iff in H. destruct H.
+      -- exists froms, tos. destruct H. inversion H0. subst. apply WF.find_mapsto_iff. assumption.
+      -- firstorder.
+    + firstorder. bdestruct ((fst x) =? node).
+      -- subst. exists ((l, whose) :: froms), tos. apply WF.add_mapsto_iff. left. split. 
+        ++ reflexivity.
+        ++ destruct x. simpl in *. apply WF.find_mapsto_iff in isIn. assert ((froms, label, tos) = (x0, a, x1)). {
+          apply (WF.MapsTo_fun isIn).
+          assumption.
+        }
+        inversion H0. firstorder.
+      -- exists x0, x1. apply WF.add_mapsto_iff. right. split.
+        ++ lia.
+        ++ assumption.
+  - reflexivity. *)
+Admitted.
+
+
+Lemma _updAdj_filter_clearSucc_does_not_change_lab_nodes : forall (A B : Type) (node : Node) (fromss : Adj B)  (ig : IG A B) (x : LNode A),  
+  In x
+(IG_labNodes
+(_updAdj (filter (fun '(_, n) => negb (n =? node)) fromss) (fun (_ : B) (y : Context' A B) => _clearSucc node y)
+(ig))) <-> In x (IG_labNodes ig).
+Proof.
+  (* intros. unfold _updAdj.
+  induction adj.
+  - simpl. reflexivity.
+  - simpl. destruct a. rewrite _updateEntry_addPred_does_not_change_lab_nodes. rewrite <- IHadj. reflexivity. *)
+Admitted.
+
+
+
+Lemma _updateEntry_filter_clearPred_does_not_change_lab_nodes : forall (A B : Type) (node : Node) (whose : Node) (l : B) (ig : IG A B) (x : LNode A),
+  In x (IG_labNodes (_updateEntry node (_addPred whose l) ig)) <-> In x (IG_labNodes ig).    
+Proof.
+
+
+  (* intros. unfold _updateEntry. unfold _addPred. 
+  destruct (NatMap.find node ig) eqn:isIn.
+  - destruct c as [[froms label] tos]. rewrite !_In_labNodes_is_InMap. split; intros.
+    + destruct H as [fromss [toss H]]. apply WF.add_mapsto_iff in H. destruct H.
+      -- exists froms, tos. destruct H. inversion H0. subst. apply WF.find_mapsto_iff. assumption.
+      -- firstorder.
+    + firstorder. bdestruct ((fst x) =? node).
+      -- subst. exists ((l, whose) :: froms), tos. apply WF.add_mapsto_iff. left. split. 
+        ++ reflexivity.
+        ++ destruct x. simpl in *. apply WF.find_mapsto_iff in isIn. assert ((froms, label, tos) = (x0, a, x1)). {
+          apply (WF.MapsTo_fun isIn).
+          assumption.
+        }
+        inversion H0. firstorder.
+      -- exists x0, x1. apply WF.add_mapsto_iff. right. split.
+        ++ lia.
+        ++ assumption.
+  - reflexivity. *)
+Admitted.
+
+
+Lemma _updAdj_filter_clearPred_does_not_change_lab_nodes : forall (A B : Type) (node : Node) (toss : Adj B)  (ig : IG A B) (x : LNode A), 
+  In x
+(IG_labNodes
+(_updAdj (filter (fun '(_, n) => negb (n =? node)) toss) (fun (_ : B) (y : Context' A B) => _clearPred node y)
+(ig))) <-> In x (IG_labNodes ig).
+Proof.
+  (* intros. unfold _updAdj.
+  induction adj.
+  - simpl. reflexivity.
+  - simpl. destruct a. rewrite _updateEntry_addPred_does_not_change_lab_nodes. rewrite <- IHadj. reflexivity. *)
+Admitted.
+
+
+
+
+
+Lemma IG_match_removes_node : forall (A B : Type) (query : Node) (mContext : MContext A B) (ig rest : IG A B),
+  IG_match query ig = (mContext, rest) -> 
+  forall label, not (In (query, label) (IG_labNodes rest)).
+Proof.
+  intros. unfold not. intros.
+  unfold IG_match in H. destruct (NatMap.find query ig) eqn:HH.
+  - unfold _cleanSplit in H. destruct c as [[fromss l] toss]. inversion H. clear H H2. rewrite <- H3 in H0. clear H3.
+    apply _updAdj_filter_clearPred_does_not_change_lab_nodes in H0.
+    apply _updAdj_filter_clearSucc_does_not_change_lab_nodes in H0.
+
+    apply _In_labNodes_is_InMap in H0. destruct H0 as [fromsss [tosss H0]]. simpl in H0.
+    apply WF.remove_mapsto_iff in H0. destruct H0.
+    destruct H. reflexivity.
+  
+  - inversion H. subst. apply WF.not_find_in_iff in HH. apply _In_labNodes_is_InMap in H0.
+    assert (NatMap.In query rest). {
+      firstorder.
+    }
+    auto.
+Qed.
+
+
+
+
+Lemma IG_match_just_removes_node : forall (A B : Type) (query hit : Node) (label : A) (ig rest : IG A B) (froms tos : Adj B) (x : LNode A),
+  IG_match query ig = (Some (froms, hit, label, tos), rest) -> 
+  In x (IG_labNodes ig) <-> In x ((hit, label) :: IG_labNodes rest). 
+Proof.
+  intros. simpl.
+  unfold IG_match in H. destruct (NatMap.find query ig) eqn:HH.
+  - unfold _cleanSplit in H. destruct c as [[fromss l] toss]. inversion H. subst.
+    split; intros.
+    + bdestruct (hit =? fst x).
+      -- destruct x.  subst. left. f_equal. apply _In_labNodes_is_InMap in H0. simpl in H0. firstorder. apply WF.find_mapsto_iff in HH.
+        assert ((fromss, label, tos) = (x, a, x0)). {
+          apply (WF.MapsTo_fun HH H0).
+        }
+        inversion H1. reflexivity.
+      -- right. apply _updAdj_filter_clearPred_does_not_change_lab_nodes. apply _updAdj_filter_clearSucc_does_not_change_lab_nodes.
+        apply _In_labNodes_is_InMap. apply _In_labNodes_is_InMap in H0. firstorder. exists x0, x1.
+        apply WF.remove_mapsto_iff. split.
+        ++ assumption.
+        ++ assumption.
+    + destruct H0.
+      -- subst. apply WF.find_mapsto_iff in HH. apply _In_labNodes_is_InMap. exists fromss, tos. assumption.
+      -- apply _updAdj_filter_clearPred_does_not_change_lab_nodes in H0. apply _updAdj_filter_clearSucc_does_not_change_lab_nodes in H0.
+        apply _In_labNodes_is_InMap in H0. apply _In_labNodes_is_InMap. firstorder. exists x0, x1. apply WF.remove_mapsto_iff in H0.
+        destruct H0. assumption.
+ 
+
+  - inversion H.
+Qed.
+
+
+
+
+  
+  
+  
 
 
 Lemma _insEdge_does_not_add_node : forall (A B : Type) (edge : LEdge B) (ig : IG A B) (x : LNode A),
   In x (IG_labNodes (_insEdge edge ig)) <-> In x (IG_labNodes ig).
 Proof.
-Admitted.
-  (* intros. unfold _insEdge. destruct edge.
-  destruct (NatMap.mem (elt:=NatSet.t * NatSet.t) n ig && NatMap.mem (elt:=NatSet.t * NatSet.t) n0 ig) eqn:H0.
-  - rewrite _updateEntry_does_not_change_key_set.
-    rewrite _updateEntry_does_not_change_key_set.
-    reflexivity.
+  intros. unfold _insEdge. destruct edge as [[from to] label].
+  destruct (IG_match from ig) eqn:HH.
+  destruct m as [[[[froms n] l] tos] | ].
+  - rewrite IG_add_adds_node. destruct (NatMap.mem from i) eqn:HHH.
+    + exfalso. apply IG_match_returns_node in HH as HHHH. subst.
+      apply  WF.mem_in_iff in HHH.
+      
+      assert (exists c, NatMap.MapsTo n c i). {
+        firstorder.
+      }
+      destruct H as [[[fromss node] toss] H].
+
+      assert (In (n, node) (IG_labNodes i)). {
+        apply _In_labNodes_is_InMap. firstorder.
+      }
+
+      eapply IG_match_removes_node in HH.
+      unfold not in HH. apply HH. apply H0.
+
+
+    + simpl. apply IG_match_returns_node in HH as HHHH. subst. apply (IG_match_just_removes_node _ _ _ _ _ _ _ _ _ x) in HH. rewrite HH. simpl. reflexivity.
   - reflexivity.
-Qed. *)
+Qed.
+
+
+
+
+
+
+
+
+
+
+
 
 
 Lemma _insEdges_does_not_add_nodes : forall (A B : Type) (edges : list (LEdge B)) (ig : IG A B) (x : LNode A), 
@@ -159,26 +519,6 @@ Proof.
   - simpl. reflexivity.
   - simpl. rewrite _insEdge_does_not_add_node. rewrite IHedges. reflexivity.
 Qed. 
-
-
-Lemma _insNode_any_ins_node : forall (A B : Type) (node : LNode A) (ig : IG A B) (x : LNode A),
-  In x (IG_labNodes (_insNode node ig)) <-> In x (node :: IG_labNodes ig).
-Proof.
-Admitted.
-  (* intros. simpl. unfold _insNode.
-  rewrite _In_labNodes_is_InMap. rewrite WF.add_mapsto_iff.
-  rewrite _In_labNodes_is_InMap.
-  reflexivity.
-Qed. *)
-
-
-Lemma _insNodes_any_ins_all_nodes : forall (A B : Type) (nodes : list (LNode A)) (ig : IG A B) (x : LNode A),
-  In x (IG_labNodes (_insNodes nodes ig)) <-> In x (nodes ++ IG_labNodes ig).
-Proof.
-  intros. induction nodes.
-    - simpl. reflexivity.
-    - simpl. rewrite _insNode_any_ins_node. simpl. rewrite IHnodes. reflexivity.
-Qed.
 
 Lemma _insEdge_on_empty_is_empty : forall (A B : Type) (edge : LEdge B),
   _insEdge edge (@IG_empty A B)= IG_empty. 
@@ -204,11 +544,20 @@ Qed.
 
 
 (* "big" statement: *)
-Theorem IG_mkGraph_any_ins_all_nodes : forall (A B : Type) (nl : list (LNode A)) (el : list (LEdge B)) (x : LNode A),
-  In x (IG_labNodes (IG_mkGraph nl el)) <-> In x nl.
+Theorem IG_mkGraph_any_ins_all_nodes : forall (A B : Type) (nodes : list (LNode A)) (edges : list (LEdge B)) (x : LNode A),
+  NoDupA (fun x y => fst x = fst y) nodes ->
+
+  In x (IG_labNodes (IG_mkGraph nodes edges)) <-> In x nodes.
 Proof.
   intros. unfold IG_mkGraph. rewrite _insEdges_does_not_add_nodes. rewrite _insNodes_any_ins_all_nodes.
-  rewrite app_nil_r. reflexivity.
+  - rewrite app_nil_r. simpl. rewrite forallb_filter_id.
+    + reflexivity.
+    + induction nodes.
+      -- simpl. reflexivity.
+      -- simpl. rewrite IHnodes.
+        ++ destruct a. simpl. reflexivity.
+        ++ inversion H. assumption.
+  - assumption.
 Qed.
 
 
